Add a scalar_tac lemma about subtypes and remove some now useless lemmas

backends/lean/Aeneas/ScalarTac/Tests.lean
@@ -1,6 +1,6 @@
 import Aeneas.ScalarTac.Lemmas
 
-namespace Aeneas.Std
+namespace Aeneas.Std.ScalarTac.Tests
 
 /-!
 # Tests
@@ -141,14 +141,13 @@ example (d i : ℕ) (h : i ≤ 256) : d * i / 8 ≤ d * 256 / 8 := by
   apply Nat.div_le_div_right
   scalar_tac +nonLin
 
-/- A bug used to make this fail -/
 example
   (i1 i2 : U16)
   (i1_post_2 : (↑i1 : ℕ) < 3329)
   (i2_post_2 : (↑i2 : ℕ) < 3329) :
   i1.val * i2.val ≤ U32.max
   := by
-  scalar_tac +fastSaturate
+  scalar_tac
 
 /- This example exhibited an "unknown free variable" bug because expressions
    containing free variables were not properly ignored. -/
@@ -160,4 +159,13 @@ example
   := by
   scalar_tac
 
-end Aeneas.Std
+
+def inv (x : Nat) : Prop := 0 < x ∧ x % 2 = 0
+@[scalar_tac inv x]
+theorem inv_imp (x : Nat) (h : inv x) : 0 < x ∧ x % 2 = 0 := by simp [inv] at h; assumption
+
+--example (x y : Nat) (h : inv x) : y % x < x := by
+--  scalar_tac
+
+
+end Aeneas.Std.ScalarTac.Tests
